Mostly fixed (one failed expectation)

src/StandardLibrary/StandardLibrary.dfy
@@ -18,7 +18,7 @@ module {:extern "STL"} StandardLibrary {
     }
   }
 
-  method {:extern} Cast<T>(x: object, ghost ensured: (T) --> bool) returns (r: Option<T>)
+  method {:extern} Cast<T>(x: object, ghost ensured: T ~> bool) returns (r: Option<T>)
     ensures r.Some? && ensured.requires(r.get) ==> ensured(r.get)
 
   datatype Result<T> = Success(value: T) | Failure(error: string)
